# 2-3 Correctness of **Horner**’s rule

> You are given the coefficents $a_0; a_1; a_2; \dots; a_n$ of a polynomial
> $$
> \begin{aligned}
>     P(x) & = \sum_{k=0}^n a_kx^k \cr
>     &=a_0+a_1x+a_2x^2+\cdots +a_{n-1}x^{n-1}+a_nx^n,
> \end{aligned}
> $$
> and you want to evaluate this polynomial for a given value of x. **Horner**'s rule** says to evalusate the polynomial according to this > parenthesization:
> $$
> P(x) = a_0 + x ( a_1 + x ( a_2 + \cdots + x ( a_{n-1} + x a_n) > \cdots )).
> $$
> The procedure **HORNER** implements **Horner**’s rule to > evaluate $P(x)$, > givem the coefficients $a_0,a_1,a_2,\dots,> a_n$ in an array $A[0:n]$ and > the value of $x$.
>
> ```cpp
> HORNER (A,n,x)
>     p=0
>     for i = n downto 0
>         p = A[i] + x * p
>     return p
> ```
>
> **a**. In terms of $\Theta$-notation, what is the tunning time of this procedure?
>
> **b**. Write pseudocode to implement the naive polynomial-evaluation algorithm that computes each term of the polynomial from scratch. What is the running time of this algorithm? How does it compare with **HORNER**?
>
> **c**. Consider the following loop invariant for the procedure **HORNER**:
>
> At the start of each iteration of the **for** loop of lines 2-3,
>
> $$
> p = \sum _{k=0}^{n-(i+1)} A[k+i+1] \cdot x^k
> $$
>
> Interpret a summation with no terms at equaling 0. Following the structure of th loop-invariant proof presented in this chapter, use this loop invariant to show that, at termination, $p = \sum _{k=0} ^{n} A[k] \cdot x^k$

## **a**

$\Theta(n)$

## **b**

pseudocode:

```cpp
naive_polynomia_evaluation (A,n,x)
    p=0
    for i = 0 to n
        term = A[i]
        for j = 1 to i
            term = term * x
        p = term + p
    return p
```

$\text{running time:} \Theta (n^2)$, **HORNER** beat it asymptotically.

## **c**

**Initialization**: $i=n, p=\sum_{k=0}^{n-(n+1)} A[k+n+1] \cdot{x^k} = 0$, loop invariant holds.

**Maintenance**: in the end of each iteration:

$$
\begin{aligned}
    p & =  A[i] + x \cdot{\sum_{k=0}^{n-(i+1)} A[k+i+1] \cdot {x^k}} \cr
    & =  A[i] + \sum_{k=0}^{n-(i+1)} A[k+i+1] \cdot{x^{k+1}}\cr
    & = A[i] \cdot{x^0} + \sum_{k=1}^{n-i} A[k+i] \cdot{x^{k}}\cr
    & = \sum_{k=0}^{n-i} A[k+i] \cdot{x^k}\cr
\end{aligned}
$$

Decrementing i preserves the loop invariant.

**Termination**: The loop terminates at $i=−1$. If we substitute,

$$
p = \sum_{k=0}^{n-(i+1)} A[k+i+1] \cdot{x^k} = \sum_{k=0}^{n} A[k] \cdot{x^k}
$$
